Stuck in simplified 2pc plan;
intended spec for Participant__PrepareIncrease would give
  is_prepared (k |-> v) (k |-> v+amnt)
as postcondition, by allocating the invariant itself. But now the
coordinator is not committing to whether it wants to Increase or
Decrease for this tid. So, it's possible for coordinator to call
PrepareDecrease concurrently with PrepareIncrease, and the naive spec
would give is_prepared (...) (k |-> v+amnt) and is_prepared (...) (k |-> v-amnt),
which is bogus. Previously, this wasn't an issue because the coordinator
was allocating the 2pc invariant, and would essentially commit to one of
the two operations for that tid and pid.

One option is to once again have the coordinator alloc the invariant,
and once again have an explicit unprepared state (which is pretty much
what it was before).
  The annoying part of that used to be that the coordinator
didn't know exactly what resources to expect, so there was that annoying
quantification over the oldvalue of that key, as well as explicit ghost
state mapping (tid,pid) -> oldvalue.
  However, I think I see how to get rid of that explicit ghost state by
keeping a copy of the invariant on the participant side, which I
previously wasn't doing.

src/program_proof/lockservice/two_pc_example.v
@@ -37,26 +37,21 @@ Section tpc_example.
 
 
 Context `{!heapG Σ}.
-Context `{!mapG Σ u64 u64}.
 
-Record TransactionC :=
-mkTransactionC {
-    heldResource:u64;
+Record TxnResourcesC :=
+mkTxnResourcesC {
+    key:u64;
     oldValue:u64;
-    operation:u64;
-    amount:u64
 }.
 
-Global Instance TransactionC_Inhabited : Inhabited TransactionC :=
-  {| inhabitant := mkTransactionC 0 0 0 0 |}.
+Global Instance TransactionC_Inhabited : Inhabited TxnResourcesC :=
+  {| inhabitant := mkTxnResourcesC 0 0 |}.
 
-#[refine] Instance TransactionC_IntoVal : into_val.IntoVal (TransactionC) :=
+#[refine] Instance TransactionC_IntoVal : into_val.IntoVal (TxnResourcesC) :=
   {
-  to_val := λ x, (#x.(heldResource), (
-          (#x.(oldValue),
-          (#x.(operation),
-          (#x.(amount), #())))))%V ;
-  IntoVal_def := mkTransactionC 0 0 0 0 ;
+  to_val := λ x, (#x.(key), (
+          (#x.(oldValue), #()))) %V ;
+  IntoVal_def := mkTxnResourcesC 0 0 ;
   IntoVal_inj := _
   }.
 Proof.
@@ -65,8 +60,6 @@ Proof.
   simpl in *. subst.
   done.
 Defined.
-
-Context `{!mapG Σ (u64*u64) (option (u64))}.
 
 Definition tpcR := csumR fracR (agreeR boolO).
 Context `{!inG Σ (gmapUR u64 tpcR)}.
@@ -77,8 +70,6 @@ mk_tpc_names  {
   tpc_state_gn : gname ;
   finish_token_gn : gname ;
 }.
-
-Print gmapUR.
 
 Implicit Type γtpc : tpc_names.
 
@@ -93,9 +84,6 @@ Definition tpc_inv_single γtpc tid R R' : iProp Σ :=
   aborted γtpc tid ∗ (R ∨ finish_token γtpc tid)
 .
 
-Definition fresh_tid γtpc (tid:u64) : iProp Σ :=
-  "Hundec" ∷ undecided_half γtpc tid.
-
 Definition txnSingleN (pid:u64) := nroot .@ "tpc" .@ pid.
 Definition is_prepared γtpc (tid pid:u64) R R' : iProp Σ := inv (txnSingleN pid) (tpc_inv_single γtpc tid R R').
 
@@ -107,46 +95,6 @@ Proof.
   iIntros.
   iMod (inv_alloc with "[-]") as "$"; last by iModIntro.
   iNext. iLeft. iFrame.
-Qed.
-
-Lemma prepared_participant_abort E γtpc tid pid R R':
-  ↑(txnSingleN pid) ⊆ E →
-  is_prepared γtpc tid pid R R' -∗
-  undecided_half γtpc tid ={E}=∗
-  aborted γtpc tid.
-Proof.
-  intros Hnamespace.
-  iIntros "#His_prep Hundec".
-  iInv "His_prep" as "Hp" "Hpclose".
-  iDestruct "Hp" as "[[>Hundec2 HR]|Hbad]".
-  {
-    iCombine "Hundec Hundec2" as "Hundec".
-    iMod (own_update _ _ {[ tid := (Cinr (to_agree false)) ]} with "Hundec") as "#Habort".
-    {
-      apply singleton_update.
-      rewrite -Cinl_op.
-      rewrite frac_op.
-      rewrite Qp_half_half.
-      by apply cmra_update_exclusive.
-    }
-    iFrame "Habort".
-    iMod ("Hpclose" with "[-]") as "_"; last by iModIntro.
-    iRight; iRight.
-    iFrame "#∗".
-  }
-  iDestruct "Hbad" as "[[>Hbad _]|[>Hbad _]]".
-  {
-    iDestruct (own_valid_2 with "Hundec Hbad") as %Hbad.
-    exfalso. rewrite singleton_op in Hbad.
-    setoid_rewrite singleton_valid in Hbad.
-    naive_solver.
-  }
-  {
-    iDestruct (own_valid_2 with "Hundec Hbad") as %Hbad.
-    exfalso. rewrite singleton_op in Hbad.
-    setoid_rewrite singleton_valid in Hbad.
-    naive_solver.
-  }
 Qed.
 
 Lemma commit_abort_false γtpc tid :
@@ -215,6 +163,31 @@ Proof.
   contradiction.
 Qed.
 
+Lemma prepared_participant_abort E γtpc tid pid R R':
+  ↑(txnSingleN pid) ⊆ E →
+  is_prepared γtpc tid pid R R' -∗
+  undecided_half γtpc tid ={E}=∗
+  aborted γtpc tid.
+Proof.
+  intros Hnamespace.
+  iIntros "#His_prep Hundec".
+  iInv "His_prep" as "Hp" "Hpclose".
+  iDestruct "Hp" as "[[>Hundec2 HR]|Hbad]".
+  {
+    iMod (undecided_abort with "Hundec Hundec2") as "#$".
+    iMod ("Hpclose" with "[-]") as "_"; last by iModIntro.
+    iRight; iRight.
+    iFrame "#∗".
+  }
+  iDestruct "Hbad" as "[[>#Hbad _]|[>#Hbad _]]".
+  {
+    iExFalso. iApply undecided_commit_false; eauto.
+  }
+  {
+    iExFalso. iApply undecided_abort_false; eauto.
+  }
+Qed.
+
 Lemma prepared_participant_finish_commit E γtpc tid pid R R':
   ↑(txnSingleN pid) ⊆ E →
   is_prepared γtpc tid pid R R' -∗ committed γtpc tid -∗ finish_token γtpc tid ={E}=∗
@@ -267,9 +240,9 @@ Qed.
 (* Proof of participant code *)
 Record participant_names :=
 mk_participant_names  {
+    ps_tpc:tpc_names ;
     ps_ghs:list (deletable_heap.gen_heapG u64 bool Σ) ;
     ps_kvs:gname ;
-    ps_kvs_phys:gname ;
 }.
 
 Implicit Type γ : participant_names.
@@ -282,12 +255,14 @@ Proof.
   intros [] [] _; auto.
 Defined.
 
-Definition kv_ctx γ (kvsM:gmap u64 u64) k : iProp Σ :=
-  k [[γ.(ps_kvs_phys)]]↦ (map_get kvsM k).1 ∗ k [[γ.(ps_kvs)]]↦{3/4} (map_get kvsM k).1 ∨
-  (Locked γ.(ps_ghs) k) ∗ k [[γ.(ps_kvs_phys)]]↦{1/2} (map_get kvsM k).1.
+Context `{!mapG Σ u64 u64}.
 
-Definition ps_mu_inv (ps:loc) γ γtpc pid : iProp Σ :=
-  ∃ (kvs_ptr txns_ptr finishedTxns_ptr lockMap_ptr:loc) (kvsM:gmap u64 u64) (txnsM:gmap u64 TransactionC)
+Definition kv_ctx γ (kvsM:gmap u64 u64) k : iProp Σ :=
+  k [[γ.(ps_kvs)]]↦{3/4} (map_get kvsM k).1 ∨
+  (Locked γ.(ps_ghs) k).
+
+Definition ps_mu_inv (ps:loc) γ pid : iProp Σ :=
+  ∃ (kvs_ptr txns_ptr finishedTxns_ptr lockMap_ptr:loc) (kvsM:gmap u64 u64) (txnsM:gmap u64 TxnResourcesC)
     (finishedTxnsM:gmap u64 bool),
 
     "Hkvs" ∷ ps ↦[ParticipantServer.S :: "kvs"] #kvs_ptr ∗
@@ -302,34 +277,31 @@ Definition ps_mu_inv (ps:loc) γ γtpc pid : iProp Σ :=
     "Hkvs_ctx" ∷ ([∗ set] k ∈ (fin_to_set u64), kv_ctx γ kvsM k) ∗
     "#HlockMap" ∷ is_lockMap lockMap_ptr γ.(ps_ghs) (fin_to_set u64) (λ _, True) ∗
 
-    "#Htxns_prop_pers" ∷ ([∗ map] tid ↦ txn ∈ txnsM, (prepared γtpc tid pid) ∗ (tid, pid)[[γtpc.(txn_data_gn)]]↦ro Some txn.(oldValue))∗
-    "Htxns_own" ∷ ([∗ map] tid ↦ txn ∈ txnsM, txn.(heldResource) [[γ.(ps_kvs_phys)]]↦{1/2} (word.add txn.(oldValue) txn.(amount))) ∗
-    (* TODO: need phys value to be correct *) "Htxns_own" ∷ ([∗ map] tid ↦ txn ∈ txnsM,  txn.(heldResource) [[γ.(ps_kvs_phys)]]↦{1/2} (word.add txn.(oldValue) txn.(amount))) ∗
-    "Hfinish_tok" ∷ ([∗ set] tid ∈ (fin_to_set u64), (⌜is_Some (finishedTxnsM !! tid)⌝ ∨ finish_token γtpc tid pid)) ∗
-    "Hdata_unused" ∷ ([∗ set] tid ∈ (fin_to_set u64), (⌜tid ∈ dom (gset u64) finishedTxnsM ∪ dom (gset u64) txnsM⌝ ∨ (tid,pid) [[γtpc.(txn_data_gn)]]↦ None)) ∗
+    "#Htxns_prop_pers" ∷ ([∗ map] tid ↦ txn ∈ txnsM, is_prepared γ.(ps_tpc) tid pid (txn.(key) [[γ.(ps_kvs)]]↦{3/4} txn.(oldValue)) (txn.(key) [[γ.(ps_kvs)]]↦{3/4} (map_get kvsM txn.(key)).1) ) ∗
+    "Hundec_tok" ∷ ([∗ set] tid ∈ (fin_to_set u64), (⌜tid ∈ dom (gset u64) finishedTxnsM⌝ ∨ ⌜tid ∈ dom (gset u64) txnsM⌝ ∨ undecided_half γ.(ps_tpc) tid)) ∗
+    "Hfinish_tok" ∷ ([∗ set] tid ∈ (fin_to_set u64), (⌜tid ∈ dom (gset u64) finishedTxnsM⌝ ∨ finish_token γ.(ps_tpc) tid)) ∗
     "%" ∷ ⌜(dom (gset u64) txnsM) ## dom (gset u64) finishedTxnsM⌝
 .
 
 Definition participantN := nroot .@ "participant".
 
-Definition is_participant (ps:loc) γ γtpc pid : iProp Σ :=
+Definition is_participant (ps:loc) γ pid : iProp Σ :=
   ∃ (mu:loc),
   "#Hmu" ∷ readonly (ps ↦[ParticipantServer.S :: "mu"] #mu) ∗
-  "#Hmu_inv" ∷ is_lock participantN #mu (ps_mu_inv ps γ γtpc pid)
+  "#Hmu_inv" ∷ is_lock participantN #mu (ps_mu_inv ps γ pid)
 .
 
-Lemma wp_Participant__PrepareIncrease (ps:loc) tid pid γ γtpc (key amnt:u64) :
+Lemma wp_Participant__PrepareIncrease (ps:loc) tid pid γ (key amnt:u64) :
   {{{
-       is_txn_single γtpc tid pid (λ data, data.(heldResource) [[γ.(ps_kvs)]]↦{3/4} data.(oldValue)) (λ data, key [[γ.(ps_kvs)]]↦{3/4} (word.add data.(oldValue) amnt)) ∗
-       is_participant ps γ γtpc pid
+       is_participant ps γ pid
   }}}
     ParticipantServer__PrepareIncrease #ps #tid #key #amnt
   {{{
-       (a op oldValue:u64), RET #a; ⌜a ≠ 0⌝ ∨ ⌜a = 0⌝ ∗ prepared γtpc tid pid ∗
-       (tid,pid) [[γtpc.(txn_data_gn)]]↦ro Some (mkTransactionC key oldValue op amnt)
+       (a oldv:u64), RET #a; ⌜a ≠ 0⌝ ∨ ⌜a = 0⌝ ∗
+        is_prepared γ.(ps_tpc) tid pid (key [[γ.(ps_kvs)]]↦{3/4} oldv) (key [[γ.(ps_kvs)]]↦{3/4} (word.add oldv amnt))
   }}}.
 Proof.
-  iIntros (Φ) "[#Htxn #Hps] HΦ".
+  iIntros (Φ) "#Hps HΦ".
   iNamed "Hps".
   wp_lam.
   wp_pures.
@@ -353,7 +325,7 @@ Proof.
   wp_pures.
   wp_if_destruct.
   { (* Transaction already finished *)
-    wp_loadField. wp_apply (release_spec with "[$Hmu_inv $Hmulocked Hkvs Htxns HfinishedTxns HlockMap_ptr HkvsMap HtxnsMap HfinishedTxnsMap Hkvs_ctx Htxns_own Hfinish_tok Hdata_unused]").
+    wp_loadField. wp_apply (release_spec with "[$Hmu_inv $Hmulocked Hkvs Htxns HfinishedTxns HlockMap_ptr HkvsMap HtxnsMap HfinishedTxnsMap Hkvs_ctx Hundec_tok Hfinish_tok]").
     {
       iNext. iExists _, _, _,_,_,_,_; iFrame "#∗".
       done.
@@ -381,7 +353,7 @@ Proof.
     (* Unsafe increase *)
     wp_loadField. wp_apply (wp_LockMap__Release with "[$HlockMap $Hkeylocked $Hkph]").
     wp_pures.
-    wp_loadField. wp_apply (release_spec with "[$Hmu_inv $Hmulocked Hkvs Htxns HfinishedTxns HlockMap_ptr HkvsMap HtxnsMap HfinishedTxnsMap Hkvs_ctx Htxns_own Hfinish_tok Hdata_unused]").
+    wp_loadField. wp_apply (release_spec with "[$Hmu_inv $Hmulocked Hkvs Htxns HfinishedTxns HlockMap_ptr HkvsMap HtxnsMap HfinishedTxnsMap Hkvs_ctx Hundec_tok Hfinish_tok]").
     {
       iNext. iExists _, _, _,_,_,_,_; iFrame "#∗".
       done.
@@ -395,7 +367,7 @@ Proof.
   wp_apply (wp_MapGet with "HkvsMap").
   iIntros (old_v3 ok_old_v3) "[%Hmapget_v3 HkvsMap]".
   wp_loadField.
-  wp_apply (wp_MapInsert _ _ _ _ (mkTransactionC _ _ _ _) with "HtxnsMap").
+  wp_apply (wp_MapInsert _ _ _ _ (mkTxnResourcesC _ _) with "HtxnsMap").
   { eauto. }
   iIntros "HtxnsMap".
   wp_pures.
@@ -411,12 +383,9 @@ Proof.
 
   iDestruct (big_sepS_elem_of_acc_impl key with "Hkvs_ctx") as "[Hptsto Hkvs_ctx]".
   { set_solver. }
-  iDestruct "Hptsto" as "[[Hphysptsto Hptsto]|Hbad]"; last first.
+  iDestruct "Hptsto" as "[Hptsto|Hbad]"; last first.
   { admit. (* conflict Hbad Hkeylocked *) }
-  iMod (map_update _ _ (word.add old_v4 amnt) with "[] Hphysptsto") as "[_ Hphysptsto]".
-  { admit. }
-  iDestruct "Hphysptsto" as "[Hphysptsto Hphysptsto2]".
-  iSpecialize ("Hkvs_ctx" $! (λ k, kv_ctx γ (typed_map.map_insert kvsM key (word.add old_v4 amnt)) k)%I with "[] [Hkeylocked Hphysptsto2]").
+  iSpecialize ("Hkvs_ctx" $! (λ k, kv_ctx γ (typed_map.map_insert kvsM key (word.add old_v4 amnt)) k)%I with "[] [Hkeylocked]").
   { iModIntro. iIntros.
     unfold kv_ctx.
     rewrite map_get_val.
@@ -428,40 +397,32 @@ Proof.
   {
     unfold kv_ctx.
     iRight.
-    unfold map_get, typed_map.map_insert.
-    rewrite lookup_insert.
     iFrame.
   }
 
-  (* Get finish token *)
-  iDestruct (big_sepS_elem_of_acc _ _ tid with "Hfinish_tok") as "[Hfinish_tok Hfinish_rest]".
+  (* Get unused undecided_half token *)
+  iDestruct (big_sepS_elem_of_acc_impl tid with "Hundec_tok") as "[Hundec Hundec_rest]".
   { set_solver. }
-  iDestruct "Hfinish_tok" as "[%Hbad|Hfinish_tok]".
-  { exfalso. admit. (* use Hmapget_finished and Hbad *) }
-
-  (* Get unused data token *)
-  iDestruct (big_sepS_elem_of_acc_impl tid with "Hdata_unused") as "[Hdata Hdata_rest]".
-  { set_solver. }
-  iDestruct  "Hdata" as "[%Hbad|Hdata]".
-  { exfalso. admit. (* tid can't be in either txnsM or finishedTxnsM *) }
-  iMod (participant_prepare (mkTransactionC key old_v3 (U64 1) amnt) with "Htxn Hfinish_tok [Hptsto] Hdata") as "(#Hprep & Hfinish_tok & #Hdata)".
+  iDestruct "Hundec" as "[%Hbad|[%Hbad|Hundec]]".
+  { exfalso. apply map_get_false in Hmapget_finished as [Hbad2 _].
+    apply (not_elem_of_dom finishedTxnsM) in Hbad2. set_solver. }
+  { exfalso. apply map_get_false in Hmapget as [Hbad2 _].
+    apply (not_elem_of_dom txnsM) in Hbad2. set_solver. }
+  iMod (participant_prepare with "Hundec Hptsto") as "#His_prep".
   { done. }
-  {
-    rewrite Hmapget_v3 /=.
-    iFrame.
-  }
-  iSpecialize ("Hfinish_rest" with "[Hfinish_tok]").
-  { by iRight. }
 
-  wp_loadField. wp_apply (release_spec with "[$Hmu_inv $Hmulocked Hkvs Htxns HfinishedTxns HlockMap_ptr HkvsMap HtxnsMap HfinishedTxnsMap Hkvs_ctx Hfinish_rest Hdata_rest Htxns_own Hphysptsto]").
+  wp_loadField. wp_apply (release_spec with "[$Hmu_inv $Hmulocked Hkvs Htxns HfinishedTxns HlockMap_ptr HkvsMap HtxnsMap HfinishedTxnsMap Hkvs_ctx Hundec_rest Hfinish_tok]").
   {
     iNext. iExists _, _, _,_,_,_,_; iFrame "HkvsMap HtxnsMap #∗".
-    (* TODO: combine into one big_sepM *)
     iSplitL "".
     { (* Need to have all prepared tokens *)
       iApply big_sepM_insert.
       { apply map_get_false in Hmapget. naive_solver. }
-      iFrame "#".
+      rewrite Hmapget_v3.
+      simpl.
+      iFrame "His_prep".
+      iApply (big_sepM_impl with "Htxns_prop_pers").
+      iModIntro. iIntros.
     }
     iSplitL "Htxns_own Hphysptsto".
     {
